config_coq.v
@@ -8,10 +8,14 @@ Require Import parametes_coq.
 
 Module  Config.
   Import parameters.
-  Inductive ConsCls := |ec |cc | sc . (*seeds of the set of relations *)
-  Record op_cls : Set := {op:OperName; τ:ConsCls}.  (*An operation tagged with its consistency class*)
+  Inductive ConsCls:Type :=
+  |ec: ConsCls
+  |cc: ConsCls
+  |sc: ConsCls.
+  
+  Record op_cls : Set := mkop_cls {op:OperName; τ:ConsCls}.  (*An operation tagged with its consistency class*)
   Definition session := list op_cls. 
-  Record Soup_Ing : Set := {s:SessID; i:SeqNo; σ:session}. (*ingredients in Session Soup*)
+  Record Soup_Ing : Set := mkSoup_Ing{s:SessID; i:SeqNo; σ:session}. (*ingredients in Session Soup*)
   Definition SessSoup := (Ensemble Soup_Ing).
   Notation " S  '+soup+'  I " :=  (Union Soup_Ing S ((Singleton Soup_Ing) I))(at level 80). (*Add an ingredient to the soup*)
 (**)
