oper_semantic_coq.v
@@ -100,16 +100,15 @@ Inductive Progress (η:Effect) :  Exec->Store->SessSoup ->Exec -> Store -> SessS
 
 
 |EC: forall (τ:ConsCls) (Θ:Store)(Σ: SessSoup)(Ex Ex':Exec)(ss:SessID)(ii:SeqNo) 
-                             (opp:OperName)(r:ReplID)(ing1 ing2:Soup_Ing) (oplist:session), 
-                                                                                  (τ=ec)->
-                                                                                  [Θ |- Ex, <ss,ii,opp> ~r~> Ex', η] ->
+                             (opp:OperName)(opcls:op_cls)(r:ReplID)(ing1 ing2:Soup_Ing) (oplist:session), 
+                                                                                  (τ=ec)-> (opcls = mkop_cls opp τ) ->                                                                                                                                                                 [Θ |- Ex, <ss,ii,opp> ~r~> Ex', η] ->
                                                                                   (ing1.(s)=ss) ->
                                                                                   (ing2.(s)=ss) ->
                                                                                   (ing1.(i)=ii) ->
                                                                                   (ing2.(i)=ii+1) ->
-                                                                                  (ing2.(σ)= tail oplist) ->
-                                                                                  (ing1.(σ)=oplist)->
-                                                                                  (hd Error_opcls oplist=Build_op_cls opp τ)
+                                                                                  (ing2.(σ)= oplist) ->
+                                                                                  (ing1.(σ)= opcls::oplist)->
+                                                                                  (hd Error_opcls oplist=mkop_cls opp τ)
                                                                                                                    ->[[Ex,Θ,Σ+soup+ing1 --η-->  Ex' ,Θ ,Σ+soup+ing2 ]]                   
 
 
